CertiGC/gc_spec.v
@@ -294,7 +294,7 @@ Definition do_generation_spec :=
          fun_info_rep rsh f_info fi;
          outlier_rep outlier;
          graph_rep g;
-         do_generation_ti_rep from sh t_info ti)
+         thread_info_rep sh t_info ti)
   POST [tvoid]
     EX g' : LGraph, EX t_info': thread_info, EX roots': roots_t,
     PROP (super_compatible (g', t_info', roots') f_info outlier;
@@ -371,22 +371,20 @@ Definition resume_spec :=
   PRE [ _fi OF (tptr tuint),
         _ti OF (tptr thread_info_type)]
     PROP (readable_share rsh; writable_share sh;
-          graph_thread_info_compatible g t_info)
+          graph_thread_info_compatible g t_info;
+          graph_gen_clear g O)
     LOCAL (temp _fi fi; temp _ti ti; gvars gv)
     SEP (all_string_constants rsh gv;
          fun_info_rep rsh f_info fi;
          graph_rep g;
          thread_info_rep sh t_info ti)
   POST [tvoid]
-    EX g': LGraph, EX t_info': thread_info,
-    PROP (fun_word_size f_info <= total_space (heap_head (ti_heap t_info));
-          resume_graph_relation g g';
-          resume_thread_info_relation t_info t_info')
+    PROP (fun_word_size f_info <= total_space (heap_head (ti_heap t_info)))
     LOCAL ()
     SEP (all_string_constants rsh gv;
          fun_info_rep rsh f_info fi;
-         graph_rep g';
-         thread_info_rep sh t_info' ti).
+         graph_rep g;
+         before_gc_thread_info_rep sh t_info ti).
 
 Definition garbage_collect_spec :=
   DECLARE _garbage_collect
@@ -402,7 +400,7 @@ Definition garbage_collect_spec :=
          fun_info_rep rsh f_info fi;
          outlier_rep outlier;
          graph_rep g;
-         thread_info_rep sh t_info ti)
+         before_gc_thread_info_rep sh t_info ti)
   POST [tvoid]
     EX g': LGraph, EX t_info': thread_info, EX roots': roots_t,
     PROP (super_compatible (g', t_info', roots') f_info outlier)
