CertiGC/verif_garbage_collect.v
@@ -4,23 +4,21 @@ Lemma body_garbage_collect:
   semax_body Vprog Gprog f_garbage_collect garbage_collect_spec.
 Proof.
   start_function.
-  unfold thread_info_rep, heap_struct_rep. Intros. forward.
-  remember (ti_heap t_info) as th. remember (ti_heap_p t_info) as h.
-  destruct (heap_head_cons th) as [hs [hl [? ?]]]. rewrite H0, H1 in *. simpl tl.
-  destruct H as [[? ?] ?]. destruct (g_gen (glabel g)) eqn: ?.
-  1: exfalso; apply (g_gen_not_nil (glabel g)); assumption. rewrite <- Heqth, H0 in H.
-  simpl in H. rewrite Forall_forall in H.
-  assert (generation_space_compatible g (O, g0, hs)) by (apply H; left; reflexivity).
-  destruct H4 as [? [? ?]]. rewrite <- H4 in *. pose proof (start_isptr g0). forward.
-  forward. rewrite upd_Znth0, sublist_1_cons, Zlength_cons, sublist_same by omega.
-  forward_for_simple_bound
-    11
-    (EX i: Z, EX g_tinfo_roots: LGraph * thread_info * roots_t,
-     PROP (super_compatible g_tinfo_roots f_info outlier)
-     LOCAL (temp _h h; gvars gv)
-     SEP (all_string_constants rsh gv;
-          fun_info_rep rsh f_info fi;
-          outlier_rep outlier;
-          graph_rep (fst (fst g_tinfo_roots));
-          thread_info_rep sh (snd (fst g_tinfo_roots)) ti)).
+  unfold before_gc_thread_info_rep, heap_struct_rep. Intros. forward. pose proof H.
+  destruct H0 as [? _]. pose proof (gt_gs_compatible _ _ H0 _ (graph_has_gen_O _)).
+  destruct H1 as [? [? ?]].
+  replace (heap_head (ti_heap t_info)) with (nth_space t_info 0) by
+      (destruct (heap_head_cons (ti_heap t_info)) as [hs [hl [? ?]]];
+       unfold nth_space; rewrite H4, H5; simpl; reflexivity).
+  assert (isptr (space_start (nth_space t_info 0))) by
+      (rewrite <- H1; apply start_isptr). do 2 forward. deadvars!.
+  rewrite upd_Znth0, sublist_1_cons, Zlength_cons, sublist_same by omega.
+  fold (space_tri (nth_space t_info 0)). rewrite <- map_cons.
+  replace (nth_space t_info 0 :: tl (spaces (ti_heap t_info))) with
+      (spaces (ti_heap t_info)) by
+      (destruct (heap_head_cons (ti_heap t_info)) as [hs [hl [? ?]]];
+       unfold nth_space; rewrite H5; simpl; reflexivity).
+  gather_SEP 4 5 6. replace_SEP 0 (thread_info_rep sh t_info ti) by
+      (unfold thread_info_rep, heap_struct_rep; entailer! ;
+       do 2 (unfold_data_at 1%nat); cancel).
 Abort.
