CertiGC/verif_resume.v
@@ -1,41 +1,23 @@
 Require Import RamifyCoq.CertiGC.gc_spec.
 
-Lemma reset_0_graph_rep_eq: forall (g: LGraph) g0 l,
-    g_gen (glabel g) = g0 :: l ->
-    iter_sepcon (nat_seq 1 (length l)) (generation_rep g) = 
-    graph_rep (reset_nth_gen_graph 0 g).
-Proof.
-  intros. unfold graph_rep. unfold reset_nth_gen_graph at 1. simpl. rewrite H. simpl.
-  unfold generation_rep at 2. unfold reset_nth_gen_graph at 1. unfold nth_gen at 1.
-  simpl. rewrite H. simpl. rewrite emp_sepcon. apply iter_sepcon_func_strong. intros.
-  rewrite nat_seq_In_iff in H0. unfold generation_rep. unfold nth_sh.
-  replace (nth_gen (reset_nth_gen_graph 0 g) x) with (nth_gen g x).
-  - apply iter_sepcon_func_strong. intros. apply list_in_map_inv in H1.
-    destruct H1 as [n [? ?]]. subst x0. unfold vertex_rep. f_equal.
-    + apply vertex_address_reset.
-    + apply make_fields_reset.
-  - unfold nth_gen. simpl. rewrite H. simpl. destruct x; [exfalso; omega|reflexivity].
-Qed.
-
 Lemma body_resume: semax_body Vprog Gprog f_resume resume_spec.
 Proof.
   start_function.
-  unfold thread_info_rep. Intros. unfold heap_struct_rep.
+  unfold thread_info_rep, heap_struct_rep. Intros.
   forward. unfold fun_info_rep. forward. 1: entailer!. rewrite Znth_0_cons.
   replace_SEP 1 (fun_info_rep rsh f_info fi) by (unfold fun_info_rep; entailer!).
   forward_if True.
   - forward; entailer!.
-  - remember (ti_heap_p t_info). rewrite (data_at_isptr sh heap_type). Intros.
-    exfalso. destruct t_info. simpl in *. subst. contradiction.
-  - destruct H. destruct (g_gen (glabel g)) eqn: ?.
-    1: exfalso; apply (g_gen_not_nil (glabel g)); assumption.
-    remember (ti_heap_p t_info) as h. remember (ti_heap t_info) as th.
-    destruct (heap_head_cons th) as [hs [hl [? ?]]]. rewrite H1, H2 in *. simpl in H.
-    rewrite Forall_forall in H. assert (generation_space_compatible g (O, g0, hs)). {
-      apply H; left; reflexivity. } destruct H3 as [? [? ?]]. rewrite <- H3 in *.
-    pose proof (start_isptr g0). forward. rewrite Znth_0_cons. forward.
-    rewrite Znth_0_cons. simpl tl. remember (start_address g0).
-    destruct v; try contradiction.
+  - remember (ti_heap_p t_info). rewrite (data_at_isptr sh heap_type).
+    Intros. exfalso. destruct t_info. simpl in *. subst. contradiction.
+  - Intros. destruct (heap_head_cons (ti_heap t_info)) as [hs [hl [? ?]]]. 
+    rewrite H1, <- H2, map_cons.
+    destruct (gt_gs_compatible _ _ H _ (graph_has_gen_O _)) as [? [? ?]].
+    assert (isptr (space_start (heap_head (ti_heap t_info)))). {
+      rewrite H2. unfold nth_space in H3. rewrite H1 in H3. simpl in H3.
+      rewrite <- H3. apply start_isptr. } unfold space_tri at 1. do 2 forward.
+    rewrite Znth_0_cons.
+    destruct (space_start (heap_head (ti_heap t_info))) eqn:? ; try contradiction.
     forward_if (fun_word_size f_info <= total_space hs).
     + unfold denote_tc_samebase. simpl. entailer!.
     + unfold all_string_constants. Intros.
@@ -49,40 +31,29 @@ Proof.
       rewrite (Ptrofs.signed_repr 4) in H7 by rep_omega.
       rewrite Ptrofs.signed_repr in H7 by (apply total_space_signed_range).
       rewrite WORD_SIZE_eq in H7. rewrite Z.mul_comm, Z.quot_mul in H7 by omega.
-      rewrite ptrofs_to_int_repr in H7. hnf in H7. unfold strict_bool_val in H7.
-      simpl in H7.
-      remember (Int.ltu (Int.repr (total_space h)) (Int.repr (fun_word_size f_info))).
-      unfold Val.of_bool in H7. destruct b; simpl in H7. 1: discriminate.
-      symmetry in Heqb. apply ltu_repr_false in Heqb;
-                          [omega | apply total_space_range | apply word_size_range].
-    + Intros. forward. forward. deadvars!. unfold graph_rep. rewrite Heql.
-      simpl length. unfold nat_inc_list. simpl nat_seq. simpl iter_sepcon. Intros.
-      sep_apply (generation_rep_data_at_ g O  (graph_has_gen_O g)).
-      unfold graph_gen_size, nth_gen. rewrite Heql. simpl nth. rewrite H5.
-      unfold gen_start, nth_gen. if_tac. 2: exfalso; apply H8; apply graph_has_gen_O.
-      clear H8. rewrite Heql. simpl nth. rewrite <- Heqv.
-      unfold heap_rest_rep. rewrite H1. simpl iter_sepcon. Intros.
-      unfold space_rest_rep at 1. rewrite <- H3, <- H4, if_false. 2: discriminate.
-      freeze [1; 2; 3; 4; 5] FR. gather_SEP 1 2.
-      replace (nth_sh g 0) with (generation_sh g0) by
-          (unfold nth_sh, nth_gen; rewrite Heql; simpl; reflexivity).
-      remember (generation_sh g0) as sh0.
-      assert (0 <= used_space hs <= total_space hs) by (apply space_order).
-      rewrite <- (data_at__tarray_value
-                    sh0 (total_space hs) (used_space hs) (Vptr b i) H8). thaw FR.
-      forward. Exists (reset_nth_gen_graph O g) (reset_nth_heap_thread_info O t_info).
-      entailer!.
-      1: split; [apply reset_resume_g_relation | apply reset_resume_t_relation].
-      rewrite (reset_0_graph_rep_eq _ _ _ Heql). entailer!.
-      unfold reset_nth_heap_thread_info. unfold thread_info_rep. simpl.
-      rewrite H1. simpl tl. unfold heap_rest_rep. simpl.
-      rewrite H1. simpl iter_sepcon. cancel.
-      destruct (heap_head_cons (reset_nth_heap 0 (ti_heap t_info))) as [rs [rl [? ?]]].
-      rewrite H14. unfold reset_nth_heap in H2. simpl in H2. rewrite H1 in H2.
-      inversion H2. subst rl. clear rs H2 H14 H16.
-      remember (heap_head (ti_heap t_info)).
-      unfold reset_space. simpl. unfold space_rest_rep. simpl. rewrite <- H3.
-      if_tac. 1: discriminate.
-      rewrite H4, Z.mul_0_r, Z.sub_0_r, isptr_offset_val_zero by (exact I).
-      unfold heap_struct_rep. entailer!.
+      rewrite ptrofs_to_int_repr in H7. hnf in H7.
+      destruct (Int.ltu (Int.repr (total_space h))
+                        (Int.repr (fun_word_size f_info))) eqn:? ; simpl in H7.
+      1: inversion H7. apply ltu_repr_false in Heqb;
+                         [omega | apply total_space_range | apply word_size_range].
+    + rewrite <- Heqv in *. red in H0. rewrite H0 in H5.
+      unfold previous_vertices_size in H5. simpl in H5. unfold nth_space in H5.
+      rewrite H1 in H5. simpl in H5. rewrite <- H2 in H5.
+      replace_SEP
+        4 (heap_struct_rep
+             sh ((space_start (heap_head (ti_heap t_info)),
+                  (offset_val (WORD_SIZE * used_space (heap_head (ti_heap t_info)))
+                              (space_start (heap_head (ti_heap t_info))),
+                   offset_val (WORD_SIZE * total_space (heap_head (ti_heap t_info)))
+                              (space_start (heap_head (ti_heap t_info)))))
+                   :: map space_tri hl) (ti_heap_p t_info)) by
+          (unfold heap_struct_rep; entailer!). do 3 forward.
+      unfold before_gc_thread_info_rep. rewrite !heap_struct_rep_eq. rewrite <- H5.
+      replace (WORD_SIZE * 0)%Z with 0 by omega.
+      rewrite !isptr_offset_val_zero by assumption. cancel. rewrite H1. simpl tl.
+      assert (12 = Zlength (map space_tri hl) + 1). {
+        pose proof (spaces_size (ti_heap t_info)). rewrite MAX_SPACES_eq in H2.
+        rewrite <- H2, H1, Zlength_cons, Zlength_map. omega. } rewrite !H2.
+      rewrite !data_at_tarray_split_1 by reflexivity. cancel.
+      do 2 (unfold_data_at 1%nat). cancel.
 Qed.
